verif/btrees/verif_splitnode.v
@@ -18,26 +18,6 @@ Require Import verif_newnode.
 Require Import verif_findindex.
 Require Import index.
 
-Lemma numKeys_nth_first: forall (X:Type) (le:listentry X) i,
-    (i <= numKeys_le le)%nat ->
-    numKeys_le (nth_first_le le i) = i.
-Proof.
-  intros. generalize dependent i.
-  induction le; intros.
-  - destruct i; simpl. auto. simpl in H. omega.
-  - destruct i.
-    + simpl. auto.
-    + simpl. apply f_equal. apply IHle. simpl in H. omega.
-Qed.
-
-Lemma length_to_list: forall le,
-    Zlength (le_to_list le) = Z.of_nat (numKeys_le le).
-Proof.
-  intros. induction le.
-  - simpl. apply Zlength_nil.
-  - simpl. rewrite Zlength_cons. rewrite Zpos_P_of_succ_nat. apply f_equal. auto.
-Qed.
-
 Lemma upd_Znth_twice: forall (A:Type) l i (x:A) x',
           0 <= i < Zlength l -> 
           upd_Znth i (upd_Znth i l x) x' = upd_Znth i l x'.
@@ -66,6 +46,7 @@ Admitted.
 Lemma body_splitnode: semax_body Vprog Gprog f_splitnode splitnode_spec.
 Proof.
   start_function.
+  rename H1 into LEAFENTRY.
   destruct n as [ptr0 le isLeaf First Last nval].
   pose(n:=btnode val ptr0 le isLeaf First Last nval).
   destruct(entry_val_rep e) as [keyrepr coprepr] eqn:HEVR.
@@ -116,12 +97,13 @@ Proof.
     { simpl in INRANGE. omega. }
     replace (findRecordIndex' le k (index.ip 0)) with (index.ip fri). simpl.
     gather_SEP 0 1 2 3.
-    pose (nright := btnode val ptr0 le true First false nval).
-    replace_SEP 0 (btnode_rep nright).
-    { entailer!. rewrite unfold_btnode_rep with (n:=nright). unfold nright.
+    pose (nleft := btnode val ptr0 le true First false nval).
+    replace_SEP 0 (btnode_rep nleft).
+    { entailer!. rewrite unfold_btnode_rep with (n:=nleft). unfold nleft.
       Exists ent_end. cancel. } clear ent_end. fold tentry.
     assert(ENTRY: exists ke ve xe, e = keyval val ke ve xe). (* the entry to be inserted at a leaf must be keyval *)
-    { admit. }
+    { destruct e. eauto. simpl in LEAFENTRY.
+      rewrite LEAF in LEAFENTRY. exfalso. rewrite LEAFENTRY. auto. }
     destruct ENTRY as [ke [ve [xe ENTRY]]].
     
     forward_for_simple_bound (Z.of_nat fri)
@@ -132,7 +114,7 @@ Proof.
       temp _t'1 (Vint (Int.repr (Z.of_nat fri))); temp _t'28 keyrepr;
       lvar _allEntries (tarray tentry 16) v_allEntries; temp _node nval; temp _entry pe;
       temp _isLeaf (Val.of_bool isLeaf))
-      SEP (btnode_rep nright; btnode_rep (empty_node isLeaf false Last vnewnode);
+      SEP (btnode_rep nleft; btnode_rep (empty_node isLeaf false Last vnewnode);
            data_at Tsh (tarray tentry 16) (le_to_list (nth_first_le le (Z.to_nat i))++ allent_end) v_allEntries; entry_rep e; data_at Tsh tentry (keyrepr, coprepr) pe)))%assert.
     { simpl in INRANGE. rewrite Fanout_eq in INRANGE.
       replace (Z.of_nat 15) with 15 in INRANGE. rep_omega. simpl. auto. }
@@ -140,7 +122,7 @@ Proof.
       Exists (default_val (nested_field_type (tarray (Tstruct _Entry noattr) 16) [])).
       entailer!. unfold data_at_, field_at_. entailer!. }
     {                           (* loop body *)
-      rewrite unfold_btnode_rep with (n:=nright). unfold nright.
+      rewrite unfold_btnode_rep with (n:=nleft). unfold nleft.
       Intros ent_end.
       assert(HENTRY: exists e, nth_entry_le (Z.to_nat i) le = Some e).
       { apply nth_entry_le_in_range. simpl in INRANGE. rewrite Fanout_eq in INRANGE.
@@ -148,7 +130,10 @@ Proof.
       destruct HENTRY as [ei HENTRY].
       assert (HEI: exists ki vi xi, ei = keyval val ki vi xi).
       { eapply integrity_nth_leaf. eauto. rewrite LEAF. simpl. auto. eauto. }
-      destruct HEI as [ki [vi [xi HEI]]]. subst ei.        
+      destruct HEI as [ki [vi [xi HEI]]]. subst ei.
+      assert_PROP(isptr xi).
+      { apply le_iter_sepcon_split in HENTRY. rewrite HENTRY. simpl entry_rep. entailer!. }
+      rename H5 into XIPTR.
       assert(HZNTH: forall ent_end, Znth (d:=(Vundef,inl Vundef)) i (le_to_list le ++ ent_end) = entry_val_rep (keyval val ki vi xi)).
       { intros. rewrite <- Z2Nat.id with (n:=i). apply Znth_to_list. auto. omega. }
       assert(HIRANGE: (0 <= i < 15)).
@@ -160,19 +145,34 @@ Proof.
       Opaque Znth.
       forward.                 (* allEntries[i].key = t'26 *)
       forward.                 (* t'25=node->entries[i]->ptr.record *)
-      { rewrite HZNTH. entailer!. admit. }
+      { rewrite HZNTH. entailer!. }
       rewrite HZNTH. simpl.
       forward.                  (* allEntries[i]->ptr.record=t'25 *)
       entailer!.
+      assert(XEMP: Zlength x > 0).
+      { destruct x. clear - H4 HIRANGE. simpl in H4. rewrite Fanout_eq in H4.
+        apply eq_sym in H4. apply NPeano.Nat.sub_0_le in H4. apply inj_le in H4.
+        replace (Z.of_nat (15 + 1)) with 16 in H4. rewrite Z2Nat.id in H4. rep_omega.
+        omega. simpl. auto.
+        rewrite Zlength_cons. rep_omega. }
       Exists (sublist 1 (Zlength x) x). entailer!.
-      { clear -H4. admit. }
-      rewrite unfold_btnode_rep with (n:=nright). unfold nright. Exists ent_end. cancel.
-      
+      { clear -H4 H3 XEMP.
+        destruct x.
+        - rewrite Zlength_nil in XEMP. omega.
+        - rewrite sublist_1_cons. rewrite Zlength_cons. rewrite Zsuccminusone.
+          rewrite sublist_same by omega. simpl in H4. rewrite Z2Nat.inj_add by omega.
+          simpl.
+          assert((Fanout + 1 - Z.to_nat i)%nat = S(Fanout + 1 - (Z.to_nat i + 1))) by omega.
+          rewrite H in H4. inv H4. omega. }
+      assert(INUM: (Z.to_nat i <= numKeys_le le)%nat).
+      { unfold n  in H0. simpl in H0. rewrite H0. clear -INRANGE H3.
+        simpl in INRANGE. rep_omega. }
+      rewrite unfold_btnode_rep with (n:=nleft). unfold nleft. Exists ent_end. cancel.      
       rewrite upd_Znth_twice.
-      rewrite app_Znth2. rewrite length_to_list. rewrite numKeys_nth_first. rewrite Z2Nat.id.
+      rewrite app_Znth2. rewrite le_to_list_length. rewrite numKeys_nth_first. rewrite Z2Nat.id.
       replace (i-i) with 0 by omega.
       rewrite upd_Znth_app2.
-      rewrite length_to_list. rewrite numKeys_nth_first. rewrite Z2Nat.id.
+      rewrite le_to_list_length. rewrite numKeys_nth_first. rewrite Z2Nat.id.
       replace (i-i) with 0 by omega.
       rewrite upd_Znth_same.
       unfold upd_Znth. rewrite sublist_nil. simpl.
@@ -180,44 +180,140 @@ Proof.
       rewrite sublist_split with (lo:=0) (mid:=i) (hi:=i+1).
       erewrite sublist_len_1. rewrite <- app_nil_r with (l:=le_to_list le). rewrite HZNTH. simpl.
       rewrite app_nil_r. rewrite <- app_assoc. simpl. cancel.
-      rewrite length_to_list. unfold n in H0. simpl in H0. rewrite H0. rewrite Fanout_eq.
+      rewrite le_to_list_length. unfold n in H0. simpl in H0. rewrite H0. rewrite Fanout_eq.
       replace (Z.of_nat 15) with 15. omega. simpl. auto. omega.
-      rewrite length_to_list. unfold n in H0. simpl in H0. rewrite H0. rewrite Fanout_eq.
+      rewrite le_to_list_length. unfold n in H0. simpl in H0. rewrite H0. rewrite Fanout_eq.
       replace (Z.of_nat 15) with 15. omega. simpl. auto.
-      rewrite Zlength_app. rewrite length_to_list. rewrite numKeys_nth_first.
-      rewrite Z2Nat.id. admit.
-      omega. admit.
-      omega. admit.
-      rewrite length_to_list. rewrite numKeys_nth_first.
-      rewrite Z2Nat.id. admit.
-      omega. admit.
-      omega. admit.
-      rewrite length_to_list. rewrite numKeys_nth_first. rewrite Z2Nat.id. omega. omega.
-      admit.
-      admit. }
+      rewrite Zlength_app. rewrite le_to_list_length. rewrite numKeys_nth_first.
+      rewrite Z2Nat.id. omega. 
+      omega. omega.
+      omega. omega.
+      rewrite le_to_list_length. rewrite numKeys_nth_first.
+      rewrite Z2Nat.id. omega.
+      omega. omega.
+      omega. omega.
+      rewrite le_to_list_length. rewrite numKeys_nth_first. rewrite Z2Nat.id. omega. omega.
+      omega.
+      rewrite Zlength_app. rewrite le_to_list_length. rewrite numKeys_nth_first. rewrite Z2Nat.id.
+      omega. omega. omega. }
     Intros allent_end.
     forward.                    (* t'24=entry->key *) rewrite HK. unfold key_repr.
 
     assert(FRIRANGE: (0 <= fri < 16)%nat).
     { simpl in INRANGE. rewrite Fanout_eq in INRANGE. split. omega.
-      replace (Z.of_nat 15) with 15 in INRANGE. admit. simpl. auto. }
+      replace (Z.of_nat 15) with 15 in INRANGE.
+      apply Nat2Z.inj_lt. destruct INRANGE. eapply Z.le_lt_trans with (m:=15). rep_omega.
+      simpl. omega. simpl. auto. }
     rewrite ENTRY in HEVR. simpl in HEVR. inv HEVR.
 
     Opaque Znth.
     forward.                    (* allEntries[tgtIdx]->key = t'24 *)
     forward.                    (* t'23=entry->ptr.record *)
-    { entailer!. admit. }    
     forward.                    (* allEntries[tgtIdx]->ptr.record = t'23 *)
     assert(0 <= Z.of_nat fri < Zlength (le_to_list (nth_first_le le (Z.to_nat (Z.of_nat fri))) ++ allent_end)).
-    { split. omega. rewrite Zlength_app. rewrite length_to_list.
+    { split. omega. rewrite Zlength_app. rewrite le_to_list_length.
       rewrite numKeys_nth_first. rewrite Z2Nat.id. rewrite Zlength_correct.
-      rewrite H3. admit.
-      omega. rewrite Nat2Z.id. unfold n in H0. simpl in H0. rewrite H0. rewrite Fanout_eq. omega. }
+      rewrite H3. rewrite Nat2Z.id.
+      assert(Z.of_nat(Fanout + 1 - fri) > 0).
+      { rewrite Fanout_eq. simpl in INRANGE. rewrite Nat2Z.inj_sub.
+        simpl. omega. rewrite Fanout_eq in INRANGE. simpl in INRANGE. omega. }
+      omega. omega.
+      rewrite Nat2Z.id. unfold n in H0. simpl in H0. rewrite H0. rewrite Fanout_eq. omega. }
+    rewrite upd_Znth_twice by auto. rewrite upd_Znth_same by auto.
+    deadvars!.
+    assert(FRILENGTH: Zlength (le_to_list (nth_first_le le (Z.to_nat (Z.of_nat fri)))) = Z.of_nat fri).
+    { rewrite le_to_list_length. rewrite numKeys_nth_first. rewrite Nat2Z.id. auto.
+      rewrite Nat2Z.id. unfold n in H0. simpl in H0. rewrite H0. simpl in INRANGE. omega. }
+    unfold upd_Znth. rewrite sublist_app1 by (try rep_omega; rewrite FRILENGTH; rep_omega).
+    rewrite sublist_same by (try rep_omega; rewrite FRILENGTH; rep_omega).
+    rewrite sublist_app2 by (rewrite FRILENGTH; rep_omega).
+    repeat rewrite FRILENGTH.
+    replace (Z.of_nat fri + 1 - Z.of_nat fri) with 1 by rep_omega. rewrite Zlength_app.
+    rewrite FRILENGTH.
+    replace (Z.of_nat fri + Zlength allent_end - Z.of_nat fri) with (Zlength allent_end) by rep_omega.
 
-      rewrite upd_Znth_twice by auto. rewrite upd_Znth_same by auto.
+    forward_for_simple_bound (Z.of_nat(Fanout)) ( EX i:Z, EX ent_end:list (val * (val+val)), PROP() LOCAL(temp _newNode vnewnode; temp _tgtIdx (Vint (Int.repr (Z.of_nat fri))); lvar _allEntries (tarray tentry 16) v_allEntries; temp _node nval; temp _entry pe) SEP(btnode_rep nleft; btnode_rep (empty_node true false Last vnewnode);data_at Tsh tentry (Vint (Int.repr (k_ k)), inr xe) pe; data_at Tsh (tarray tentry 16) (le_to_list (nth_first_le le (Z.to_nat (Z.of_nat fri))) ++ (Vint (Int.repr (k_ k)), inr (force_val (sem_cast_pointer xe))) :: le_to_list(suble (S fri) (S (Z.to_nat i)) le) ++ ent_end) v_allEntries; entry_rep(keyval val ke ve xe)))%assert.
 
-    admit.                      (* second loop *)
+    { simpl in INRANGE. rewrite Fanout_eq in INRANGE.
+      replace (Z.of_nat 15) with 15 in INRANGE.
+      rewrite Fanout_eq. simpl. rep_omega. simpl. auto. }
+    abbreviate_semax.
+    {                           (* second loop *)
+      forward.                  (* i=tgtidx *)
+      Exists (Z.of_nat(fri)). Exists ( sublist 1 (Zlength allent_end) allent_end).
+      entailer!.
+      simpl in INRANGE. rep_omega.
+      rewrite Nat2Z.id. rewrite suble_nil. cancel. }
+    {                           (* loop body *)
+      admit. }
+    Intros ent_end.
+    deadvars!.
+    pose (e:=keyval val ke ve xe).
+    rewrite unfold_btnode_rep with (n:=nleft).
+    unfold nleft. Intros ent_end0.
+    forward.                    (* node->numKeys=8 *)
+    forward_if (PROP ( )
+    LOCAL (temp _newNode vnewnode; temp _tgtIdx (Vint (Int.repr (Z.of_nat fri)));
+           lvar _allEntries (tarray tentry 16) v_allEntries; temp _node nval; temp _entry pe)
+    SEP (btnode_rep (splitnode_left n e); btnode_rep (empty_node true false Last vnewnode);
+         data_at Tsh tentry (Vint (Int.repr (k_ k)), inr xe) pe;
+         data_at Tsh (tarray tentry 16) (le_to_list (nth_first_le le (Z.to_nat (Z.of_nat fri))) ++ (Vint (Int.repr (k_ k)), inr (force_val (sem_cast_pointer xe))) :: le_to_list (suble (S fri) (S (Z.to_nat (Z.of_nat Fanout))) le) ++ ent_end) v_allEntries)). (* we might still have entry_rep e if it wasnt in the first node *)
+    {                           (* fri < 8 *)
+      admit. }
+    {                           (* fri >= 8 *)
+      admit. }
+    forward_for_simple_bound (Z.of_nat(Fanout) + 1)
+    (EX i:Z, (PROP ( )
+     LOCAL (temp _newNode vnewnode; temp _tgtIdx (Vint (Int.repr (Z.of_nat fri)));
+            lvar _allEntries (tarray tentry 16) v_allEntries; temp _node nval; temp _entry pe)
+     SEP (btnode_rep (splitnode_left n e);
+          btnode_rep (btnode val None (suble Middle (Z.to_nat i) (insert_le le e)) true false Last vnewnode);
+          data_at Tsh tentry (Vint (Int.repr (k_ k)), inr xe) pe;
+          data_at Tsh (tarray tentry 16) (le_to_list (nth_first_le le (Z.to_nat (Z.of_nat fri))) ++ (Vint (Int.repr (k_ k)), inr (force_val (sem_cast_pointer xe))) :: le_to_list (suble (S fri) (S (Z.to_nat (Z.of_nat Fanout))) le) ++ ent_end) v_allEntries)))%assert.
+    { rewrite Fanout_eq. simpl. rep_omega. }
+    { rewrite Fanout_eq. simpl. rep_omega. }
+    { entailer!. rewrite Middle_eq. rewrite suble_nil. unfold empty_node. cancel. }
+    {                           (* loop body *)
+      admit. }
+    rewrite unfold_btnode_rep with (n:=(btnode val None (suble Middle (Z.to_nat (Z.of_nat Fanout + 1)) (insert_le le e)) true false Last vnewnode)).
+    Intros ent_end1. simpl.
+    forward.                    (* newnode->numKeys=15+1-8 *)
+    Intros. gather_SEP 1 2 3 4.
+    replace_SEP 0 (btnode_rep (splitnode_leafnode le e vnewnode Last)).
+    { entailer!. rewrite unfold_btnode_rep. simpl. Exists ent_end1.
+      
+      assert(HSUB: suble Middle (Z.to_nat (Z.of_nat Fanout + 1)) (insert_le le e) = skipn_le (insert_le le e) Middle).
+      { apply suble_skip. rewrite numKeys_le_insert. unfold n in H0. simpl in H0. rewrite H0.
+        rewrite Fanout_eq. simpl. auto. }
+      rewrite HSUB. cancel.
+      rewrite numKeys_le_skipn. rewrite numKeys_le_insert. unfold n in H0. simpl in H0. rewrite H0.
+      rewrite Fanout_eq. rewrite Middle_eq. simpl. cancel. }
+    replace_SEP 1 (btnode_rep (splitnode_left n e)).
+    { entailer!. }
 
+    assert(HINSERT: (le_to_list (nth_first_le le (Z.to_nat (Z.of_nat fri))) ++ (Vint (Int.repr (k_ k)), inr (force_val (sem_cast_pointer xe))) :: le_to_list (suble (S fri) (S (Z.to_nat (Z.of_nat Fanout))) le) ++ ent_end) = le_to_list (insert_le le e) ++ ent_end).
+    { admit. }
+    rewrite HINSERT.
+
+    assert(NTHENTRY: exists emid, nth_entry_le Middle (insert_le le e) = Some emid).
+    { apply nth_entry_le_in_range. unfold n in H0. simpl in H0. rewrite numKeys_le_insert.
+      rewrite H0. rewrite Middle_eq.
+      rewrite Fanout_eq. omega. }
+    destruct NTHENTRY as [emid NTHENTRY].
+    assert(HZNTH: nth_entry_le Middle (insert_le le e) = Some emid) by auto.
+    eapply Znth_to_list with (endle:=ent_end) in HZNTH.
+    rewrite Middle_eq in HZNTH. simpl in HZNTH.
+    
+    forward.                    (* t'16=allEntries[8]->key *)
+    { entailer!. rewrite HZNTH.
+      destruct emid; simpl; auto. }
+    rewrite HZNTH.
+    forward.                    (* entry->key=t'16 *)
+    forward.                    (* entry->ptr.child=newnode *)
+    forward.                    (* return *)
+    Exists vnewnode. fold e. rewrite NTHENTRY. entailer!.
+    simpl. unfold splitnode_leafnode. cancel.
+    destruct emid; simpl; cancel.
   -                             (* intern node *)
     admit.
 Admitted.
